src/StepPred.v
@@ -5,34 +5,30 @@ Require Import PredMsg.
 Set Implicit Arguments.
 
 Section GivenMsg.
-  Variable (MsgT StateT: Type).
-  Context `{HasMsg MsgT}.
+  Variable (MsgT StateT LabelT: Type).
+  Context `{HasMsg MsgT} `{HasLabel LabelT}.
 
   Definition toOrigMP (mp: MessagePool (PMsg MsgT)): MessagePool MsgT :=
     map (@pmsg_omsg _) mp.
 
-  Inductive step_pred (psys: PSystem MsgT):
-    @PState MsgT StateT -> PLabel MsgT ->
-    @PState MsgT StateT -> Prop :=
-
-  | SpSlt: forall st, step_pred psys st (emptyPLabel MsgT) st
+  Inductive step_pred0 (psys: PSystem MsgT):
+    PState MsgT -> PLabel MsgT -> PState MsgT -> Prop :=
+  | SpSlt: forall st, step_pred0 psys st (emptyPLabel MsgT) st
 
   | SpExt:
-      forall pst nst oss oims porig norig otrss (emsg: PMsg MsgT),
+      forall pst nst oss oims otrss (emsg: PMsg MsgT),
         fromExternal psys emsg = true ->
         toInternal psys emsg = true ->
         pst = {| pst_oss := oss;
                  pst_otrss := otrss;
-                 pst_msgs := oims;
-                 pst_orig := porig |} ->
+                 pst_msgs := oims |} ->
         nst = {| pst_oss := oss;
                  pst_otrss := otrss;
-                 pst_msgs := enqMP emsg oims;
-                 pst_orig := norig |} ->
-        step_pred psys pst (PlblIn emsg) nst
+                 pst_msgs := enqMP emsg oims |} ->
+        step_pred0 psys pst (PlblIn emsg) nst
 
   | SpImm:
-      forall pst nst poss noss oidx pos nos otrss poims noims porig norig
+      forall pst nst poss noss oidx pos nos otrss poims noims
              (immr: PRule MsgT) prec (rq: PMsg MsgT) (rs: PMsg MsgT),
         In oidx (indicesOf psys) ->
         In immr (psys_rules psys) ->
@@ -49,19 +45,14 @@ Section GivenMsg.
         noss = poss +[ oidx <- nos ] ->
         noims = distributeMsgs (intOuts psys (rs :: nil)) (removeMP rq poims) ->
 
-        pst = {| pst_oss := poss; pst_otrss := otrss;
-                 pst_msgs := poims; pst_orig := porig |} ->
-        nst = {| pst_oss := noss; pst_otrss := otrss;
-                 pst_msgs := noims; pst_orig := norig |} ->
+        pst = {| pst_oss := poss; pst_otrss := otrss; pst_msgs := poims |} ->
+        nst = {| pst_oss := noss; pst_otrss := otrss; pst_msgs := noims |} ->
 
-        step_pred psys pst (PlblOuts (Some immr) (rq :: nil) (rs :: nil)) nst
-                  
+        step_pred0 psys pst (PlblOuts (Some immr) (rq :: nil) (rs :: nil)) nst
+
   | SpRqFwd:
-      forall pst nst oss otrss oidx pos opred rsbf oims porig norig
+      forall pst nst oss otrss oidx pos opred rsbf oims
              (rqfwdr: PRule MsgT) prec rqff
-             (** TODO: need to know that [pmsg_omsg]s are 
-              * related in terms of the original state transition rules.
-              *)
              (rq: PMsg MsgT) (fwds: list (PMsg MsgT)),
         In oidx (indicesOf psys) ->
         In rqfwdr (psys_rules psys) ->
@@ -74,19 +65,17 @@ Section GivenMsg.
         oss@[oidx] = Some pos ->
         prec pos (getMsg rq :: nil) ->
 
-        pst = {| pst_oss := oss; pst_otrss := otrss;
-                 pst_msgs := oims; pst_orig := porig |} ->
+        pst = {| pst_oss := oss; pst_otrss := otrss; pst_msgs := oims |} ->
         nst = {| pst_oss := oss;
                  pst_otrss := otrss +[ oidx <- {| otrs_rq := rq;
                                                   otrs_opred := opred;
                                                   otrs_rsbf := rsbf |} ];
-                 pst_msgs := distributeMsgs fwds (removeMP rq oims);
-                 pst_orig := norig |} ->
+                 pst_msgs := distributeMsgs fwds (removeMP rq oims) |} ->
 
-        step_pred psys pst (PlblOuts (Some rqfwdr) (rq :: nil) fwds) nst
+        step_pred0 psys pst (PlblOuts (Some rqfwdr) (rq :: nil) fwds) nst
 
   | SpRsBack:
-      forall pst nst oss otrss oidx pos nos otrs oims porig norig
+      forall pst nst oss otrss oidx pos nos otrs oims
              (rsbackr: PRule MsgT) (rss: list (PMsg MsgT)) (rsb: PMsg MsgT),
         In oidx (indicesOf psys) ->
         In rsbackr (psys_rules psys) ->
@@ -109,14 +98,44 @@ Section GivenMsg.
 
         pst = {| pst_oss := oss;
                  pst_otrss := otrss;
-                 pst_msgs := oims;
-                 pst_orig := porig |} ->
+                 pst_msgs := oims |} ->
         nst = {| pst_oss := oss +[ oidx <- nos ];
                  pst_otrss := M.remove oidx otrss;
-                 pst_msgs := enqMP rsb (removeMsgs rss oims);
-                 pst_orig := norig |} ->
+                 pst_msgs := enqMP rsb (removeMsgs rss oims) |} ->
 
-        step_pred psys pst (PlblOuts (Some rsbackr) rss (rsb :: nil)) nst.
+        step_pred0 psys pst (PlblOuts (Some rsbackr) rss (rsb :: nil)) nst.
 
+  Variables (SysT: Type)
+            (ostep: Step SysT StateT LabelT)
+            (sysF: PSystem MsgT -> SysT)
+            (stR: StateT -> PState MsgT -> Prop)
+            (lblF: PLabel MsgT -> LabelT).
+
+  Record PStateEx :=
+    { pstx_st: StateT;
+      pstx_pst: PState MsgT;
+      pstx_r: stR pstx_st pstx_pst
+    }.
+
+  Lemma PStateEx_ext:
+    forall pstx1 pstx2,
+      pstx_st pstx1 = pstx_st pstx2 ->
+      pstx_pst pstx1 = pstx_pst pstx2 ->
+      pstx1 = pstx2.
+  Proof.
+    destruct pstx1 as [st1 pst1 r1], pstx2 as [st2 pst2 r2].
+    simpl; intros; subst.
+    replace r1 with r2 by apply proof_irrelevance.
+    reflexivity.
+  Qed.
+
+  Inductive step_pred (psys: PSystem MsgT):
+    PStateEx -> PLabel MsgT -> PStateEx -> Prop :=
+  | SpStep:
+      forall pst nst plbl,
+        ostep (sysF psys) (pstx_st pst) (lblF plbl) (pstx_st nst) ->
+        step_pred0 psys (pstx_pst pst) plbl (pstx_pst nst) ->
+        step_pred psys pst plbl nst.
+  
 End GivenMsg.
 
